10ChainedEnvironment/Chaining.thy
@@ -17,17 +17,18 @@ fun unchain_env :: "('a \<times> ptr) heap \<Rightarrow> ptr \<Rightarrow> 'a li
 
 text \<open>We map the transformation through the whole evaluation state.\<close>
 
-primrec unchain_closure :: "(ptr \<times> ptr) heap \<Rightarrow> closure\<^sub>v \<Rightarrow> closure\<^sub>h" where
+primrec unchain_closure :: "(ptr list \<times> ptr) heap \<Rightarrow> closure\<^sub>v \<Rightarrow> closure\<^sub>h" where
   "unchain_closure \<Delta> (Const\<^sub>v n) = Const\<^sub>h n"
-| "unchain_closure \<Delta> (Lam\<^sub>v p\<^sub>\<Delta> p\<^sub>\<C>) = Lam\<^sub>h (unchain_env \<Delta> p\<^sub>\<Delta>) p\<^sub>\<C>"
+| "unchain_closure \<Delta> (Lam\<^sub>v p\<^sub>\<Delta> p\<^sub>\<C> n) = Lam\<^sub>h (unchain_env \<Delta> p\<^sub>\<Delta>) p\<^sub>\<C> n"
 
-abbreviation unchain_heap :: "closure\<^sub>v heap \<Rightarrow> (ptr \<times> ptr) heap \<Rightarrow> closure\<^sub>h heap" where
+abbreviation unchain_heap :: "closure\<^sub>v heap \<Rightarrow> (ptr list \<times> ptr) heap \<Rightarrow> closure\<^sub>h heap" where
   "unchain_heap h \<Delta> \<equiv> hmap (unchain_closure \<Delta>) h"
 
-primrec unchain_frame :: "(ptr \<times> ptr) heap \<Rightarrow> (ptr \<times> nat) \<Rightarrow> (ptr list \<times> nat)" where
+primrec unchain_frame :: "(ptr list \<times> ptr) heap \<Rightarrow> (ptr \<times> nat) \<Rightarrow> (ptr list list \<times> nat)" where
   "unchain_frame \<Delta> (p\<^sub>\<Delta>, p\<^sub>\<C>) = (unchain_env \<Delta> p\<^sub>\<Delta>, p\<^sub>\<C>)"
 
-abbreviation unchain_stack :: "(ptr \<times> ptr) heap \<Rightarrow> (ptr \<times> nat) list \<Rightarrow> (ptr list \<times> nat) list" where
+abbreviation unchain_stack :: "(ptr list \<times> ptr) heap \<Rightarrow> (ptr \<times> nat) list \<Rightarrow> 
+    (ptr list list \<times> nat) list" where
   "unchain_stack \<Delta> s \<equiv> map (unchain_frame \<Delta>) s"
 
 primrec unchain_state :: "state\<^sub>v \<Rightarrow> state\<^sub>h" where
@@ -42,38 +43,38 @@ proof -
   thus ?thesis by simp
 qed
 
-lemma halloc_unchain_heap_lam [simp]: "halloc h (Lam\<^sub>v p\<^sub>\<Delta> p\<^sub>\<C>) = (h', v) \<Longrightarrow> 
-  halloc (unchain_heap h \<Delta>) (Lam\<^sub>h (unchain_env \<Delta> p\<^sub>\<Delta>) p\<^sub>\<C>) = (unchain_heap h' \<Delta>, v)"
+lemma halloc_unchain_heap_lam [simp]: "halloc h (Lam\<^sub>v p\<^sub>\<Delta> p\<^sub>\<C> n) = (h', v) \<Longrightarrow> 
+  halloc (unchain_heap h \<Delta>) (Lam\<^sub>h (unchain_env \<Delta> p\<^sub>\<Delta>) p\<^sub>\<C> n) = (unchain_heap h' \<Delta>, v)"
 proof -
-  assume "halloc h (Lam\<^sub>v p\<^sub>\<Delta> p\<^sub>\<C>) = (h', v)"
-  hence "halloc (hmap (unchain_closure \<Delta>) h) (unchain_closure \<Delta> (Lam\<^sub>v p\<^sub>\<Delta> p\<^sub>\<C>)) = 
+  assume "halloc h (Lam\<^sub>v p\<^sub>\<Delta> p\<^sub>\<C> n) = (h', v)"
+  hence "halloc (hmap (unchain_closure \<Delta>) h) (unchain_closure \<Delta> (Lam\<^sub>v p\<^sub>\<Delta> p\<^sub>\<C> n)) = 
     (hmap (unchain_closure \<Delta>) h', v)" by (metis halloc_map)
   thus ?thesis by simp
 qed
 
 text \<open>We define a set of predicates to verify our "no upward pointers" condition.\<close>
 
-abbreviation chain_structured :: "closure\<^sub>v heap \<Rightarrow> (ptr \<times> ptr) heap \<Rightarrow> bool" where
-  "chain_structured h \<Delta> \<equiv> heap_all (\<lambda>p (v, p'). p' \<le> p \<and> hcontains h v) \<Delta>"
+abbreviation chain_structured :: "closure\<^sub>v heap \<Rightarrow> (ptr list \<times> ptr) heap \<Rightarrow> bool" where
+  "chain_structured h \<Delta> \<equiv> heap_all (\<lambda>p (vs, p'). p' \<le> p \<and> list_all (hcontains h) vs) \<Delta>"
 
-primrec chained_heap_pointer :: "(ptr \<times> ptr) heap \<Rightarrow> ptr \<Rightarrow> bool" where
+primrec chained_heap_pointer :: "(ptr list \<times> ptr) heap \<Rightarrow> ptr \<Rightarrow> bool" where
   "chained_heap_pointer \<Delta> 0 = True"
 | "chained_heap_pointer \<Delta> (Suc p) = hcontains \<Delta> p"
 
-primrec chained_frame :: "(ptr \<times> ptr) heap \<Rightarrow> (ptr \<times> nat) \<Rightarrow> bool" where
+primrec chained_frame :: "(ptr list \<times> ptr) heap \<Rightarrow> (ptr \<times> nat) \<Rightarrow> bool" where
   "chained_frame \<Delta> (p\<^sub>\<Delta>, p\<^sub>\<C>) = chained_heap_pointer \<Delta> p\<^sub>\<Delta>"
 
-abbreviation chained_stack :: "(ptr \<times> ptr) heap \<Rightarrow> (ptr \<times> nat) list \<Rightarrow> bool" where
+abbreviation chained_stack :: "(ptr list \<times> ptr) heap \<Rightarrow> (ptr \<times> nat) list \<Rightarrow> bool" where
   "chained_stack \<Delta> s \<equiv> list_all (chained_frame \<Delta>) s"
 
 abbreviation chained_vals :: "closure\<^sub>v heap \<Rightarrow> ptr list \<Rightarrow> bool" where
   "chained_vals h \<V> \<equiv> list_all (hcontains h) \<V>"
 
-primrec chained_closure :: "(ptr \<times> ptr) heap \<Rightarrow> closure\<^sub>v \<Rightarrow> bool" where
+primrec chained_closure :: "(ptr list \<times> ptr) heap \<Rightarrow> closure\<^sub>v \<Rightarrow> bool" where
   "chained_closure \<Delta> (Const\<^sub>v n) = True"
-| "chained_closure \<Delta> (Lam\<^sub>v p\<^sub>\<Delta> p\<^sub>\<C>) = chained_heap_pointer \<Delta> p\<^sub>\<Delta>"
+| "chained_closure \<Delta> (Lam\<^sub>v p\<^sub>\<Delta> p\<^sub>\<C> n) = chained_heap_pointer \<Delta> p\<^sub>\<Delta>"
 
-abbreviation chained_closures :: "(ptr \<times> ptr) heap \<Rightarrow> closure\<^sub>v heap \<Rightarrow> bool" where
+abbreviation chained_closures :: "(ptr list \<times> ptr) heap \<Rightarrow> closure\<^sub>v heap \<Rightarrow> bool" where
   "chained_closures \<Delta> h \<equiv> heap_all (\<lambda>p. chained_closure \<Delta>) h"
 
 primrec chained_state :: "state\<^sub>v \<Rightarrow> bool" where
@@ -84,8 +85,8 @@ lemma chained_heap_pointer_unfold [elim]: "hcontains \<Delta> p \<Longrightarrow
   by (induction p') auto
 
 lemma lookup_unchain_env [simp]: "chain_structured h \<Delta> \<Longrightarrow> chained_heap_pointer \<Delta> p \<Longrightarrow>
-  lookup (unchain_env \<Delta> p) x = chain_lookup \<Delta> p x"
-proof (induction \<Delta> p x rule: chain_lookup.induct)
+  Option.bind (lookup (unchain_env \<Delta> p) x) (\<lambda>vs. lookup vs y) = chain_lookup \<Delta> p x y"
+proof (induction \<Delta> p x y rule: chain_lookup.induct)
   case (3 \<Delta> p x)
   obtain v p' where V: "hlookup \<Delta> p = (v, p')" by (cases "hlookup \<Delta> p")
   from 3 have "hcontains \<Delta> p" by auto
@@ -140,8 +141,8 @@ proof -
     assume X: "hcontains h x"
     show "unchain_closure \<Delta>' (hlookup h x) = unchain_closure \<Delta> (hlookup h x)" 
     proof (cases "hlookup h x")
-      case (Lam\<^sub>v p\<^sub>\<Delta> p\<^sub>\<C>)
-      with C X have "chained_closure \<Delta> (Lam\<^sub>v p\<^sub>\<Delta> p\<^sub>\<C>)" by (metis hlookup_all)
+      case (Lam\<^sub>v p\<^sub>\<Delta> p\<^sub>\<C> n)
+      with C X have "chained_closure \<Delta> (Lam\<^sub>v p\<^sub>\<Delta> p\<^sub>\<C> n)" by (metis hlookup_all)
       with S A Lam\<^sub>v show ?thesis by auto
     qed simp_all
   qed
@@ -177,12 +178,15 @@ text \<open>Completeness follows:\<close>
 theorem complete\<^sub>v [simp]: "\<C> \<tturnstile> \<Sigma>\<^sub>v \<leadsto>\<^sub>v \<Sigma>\<^sub>v' \<Longrightarrow> chained_state \<Sigma>\<^sub>v \<Longrightarrow> 
   \<C> \<tturnstile> unchain_state \<Sigma>\<^sub>v \<leadsto>\<^sub>h unchain_state \<Sigma>\<^sub>v'"
 proof (induction \<Sigma>\<^sub>v \<Sigma>\<^sub>v' rule: eval\<^sub>v.induct)
-  case (ev\<^sub>v_apply \<C> p\<^sub>\<C> h\<^sub>v v\<^sub>2 p\<^sub>\<Delta>' p\<^sub>\<C>' \<Delta>\<^sub>v v\<^sub>1 \<Delta>\<^sub>v' p\<^sub>\<Delta>'' \<V> p\<^sub>\<Delta> s\<^sub>v)
+  case (ev\<^sub>v_lookup \<C> p\<^sub>\<C> x y \<Delta> p\<^sub>\<Delta> v h \<V> s)
+  then show ?case by simp
+next
+  case (ev\<^sub>v_apply \<C> p\<^sub>\<C> h\<^sub>v v\<^sub>2 p\<^sub>\<Delta>' p\<^sub>\<C>' n \<Delta>\<^sub>v v\<^sub>1 \<Delta>\<^sub>v' p\<^sub>\<Delta>'' \<V> p\<^sub>\<Delta> s\<^sub>v)
   from ev\<^sub>v_apply have "chained_closures \<Delta>\<^sub>v h\<^sub>v \<and> hcontains h\<^sub>v v\<^sub>2" by simp
-  with ev\<^sub>v_apply have "chained_closure \<Delta>\<^sub>v (Lam\<^sub>v p\<^sub>\<Delta>' p\<^sub>\<C>')" by (metis hlookup_all)
+  with ev\<^sub>v_apply have "chained_closure \<Delta>\<^sub>v (Lam\<^sub>v p\<^sub>\<Delta>' p\<^sub>\<C>' n)" by (metis hlookup_all)
   with ev\<^sub>v_apply have "chain_structured h\<^sub>v \<Delta>\<^sub>v \<and> chained_heap_pointer \<Delta>\<^sub>v p\<^sub>\<Delta>' \<and> 
-    halloc \<Delta>\<^sub>v (v\<^sub>1, p\<^sub>\<Delta>') = (\<Delta>\<^sub>v', p\<^sub>\<Delta>'')" by auto
-  hence X: "unchain_env \<Delta>\<^sub>v' (Suc p\<^sub>\<Delta>'') = v\<^sub>1 # unchain_env \<Delta>\<^sub>v p\<^sub>\<Delta>'" by (metis unfold_unstack_list)
+    halloc \<Delta>\<^sub>v ([v\<^sub>1], p\<^sub>\<Delta>') = (\<Delta>\<^sub>v', p\<^sub>\<Delta>'')" by auto
+  hence X: "unchain_env \<Delta>\<^sub>v' (Suc p\<^sub>\<Delta>'') = [v\<^sub>1] # unchain_env \<Delta>\<^sub>v p\<^sub>\<Delta>'" by (metis unfold_unstack_list)
   from ev\<^sub>v_apply have A: "unchain_heap h\<^sub>v \<Delta>\<^sub>v' = unchain_heap h\<^sub>v \<Delta>\<^sub>v" by auto
   from ev\<^sub>v_apply have B: "unchain_env \<Delta>\<^sub>v' p\<^sub>\<Delta> = unchain_env \<Delta>\<^sub>v p\<^sub>\<Delta>" by auto
   from ev\<^sub>v_apply have "chained_stack \<Delta>\<^sub>v s\<^sub>v" by simp
@@ -194,7 +198,8 @@ proof (induction \<Sigma>\<^sub>v \<Sigma>\<^sub>v' rule: eval\<^sub>v.induct)
     by (simp add: C)
   thus ?case by simp
 next
-  case (ev\<^sub>v_pushenv \<C> p\<^sub>\<C> \<Delta>\<^sub>v v p\<^sub>\<Delta> \<Delta>\<^sub>v' p\<^sub>\<Delta>' h\<^sub>v \<V> s\<^sub>v)
+  case (ev\<^sub>v_pushenv \<C> p\<^sub>\<C> \<Delta>\<^sub>v p\<^sub>\<Delta> vs p\<^sub>\<Delta>' h\<^sub>v v \<V> s\<^sub>v)
+(*
   hence X: "unchain_heap h\<^sub>v \<Delta>\<^sub>v' = unchain_heap h\<^sub>v \<Delta>\<^sub>v" by auto
   from ev\<^sub>v_pushenv have "chained_stack \<Delta>\<^sub>v s\<^sub>v" by simp
   with ev\<^sub>v_pushenv have Y: "unchain_stack \<Delta>\<^sub>v' s\<^sub>v = unchain_stack \<Delta>\<^sub>v s\<^sub>v" by fastforce
@@ -202,13 +207,15 @@ next
     halloc \<Delta>\<^sub>v (v, p\<^sub>\<Delta>) = (\<Delta>\<^sub>v', p\<^sub>\<Delta>')" by auto
   hence "unchain_env \<Delta>\<^sub>v' (Suc p\<^sub>\<Delta>') = v # unchain_env \<Delta>\<^sub>v p\<^sub>\<Delta>" by (metis unfold_unstack_list)
   with ev\<^sub>v_pushenv X show ?case by (simp add: Y)
+*)
+  thus ?case by simp
 next
-  case (ev\<^sub>v_jump \<C> p\<^sub>\<C> h\<^sub>v v\<^sub>2 p\<^sub>\<Delta>' p\<^sub>\<C>' \<Delta>\<^sub>v v\<^sub>1 \<Delta>\<^sub>v' p\<^sub>\<Delta>'' \<V> p\<^sub>\<Delta> s\<^sub>v)
+  case (ev\<^sub>v_jump \<C> p\<^sub>\<C> h\<^sub>v v\<^sub>2 p\<^sub>\<Delta>' p\<^sub>\<C>' n \<Delta>\<^sub>v v\<^sub>1 \<Delta>\<^sub>v' p\<^sub>\<Delta>'' \<V> p\<^sub>\<Delta> s\<^sub>v)
   from ev\<^sub>v_jump have "chained_closures \<Delta>\<^sub>v h\<^sub>v \<and> hcontains h\<^sub>v v\<^sub>2" by simp
-  with ev\<^sub>v_jump have "chained_closure \<Delta>\<^sub>v (Lam\<^sub>v p\<^sub>\<Delta>' p\<^sub>\<C>')" by (metis hlookup_all)
+  with ev\<^sub>v_jump have "chained_closure \<Delta>\<^sub>v (Lam\<^sub>v p\<^sub>\<Delta>' p\<^sub>\<C>' n)" by (metis hlookup_all)
   with ev\<^sub>v_jump have "chain_structured h\<^sub>v \<Delta>\<^sub>v \<and> chained_heap_pointer \<Delta>\<^sub>v p\<^sub>\<Delta>' \<and> 
-    halloc \<Delta>\<^sub>v (v\<^sub>1, p\<^sub>\<Delta>') = (\<Delta>\<^sub>v', p\<^sub>\<Delta>'')" by auto
-  hence X: "unchain_env \<Delta>\<^sub>v' (Suc p\<^sub>\<Delta>'') = v\<^sub>1 # unchain_env \<Delta>\<^sub>v p\<^sub>\<Delta>'" by (metis unfold_unstack_list)
+    halloc \<Delta>\<^sub>v ([v\<^sub>1], p\<^sub>\<Delta>') = (\<Delta>\<^sub>v', p\<^sub>\<Delta>'')" by auto
+  hence X: "unchain_env \<Delta>\<^sub>v' (Suc p\<^sub>\<Delta>'') = [v\<^sub>1] # unchain_env \<Delta>\<^sub>v p\<^sub>\<Delta>'" by (metis unfold_unstack_list)
   from ev\<^sub>v_jump have A: "unchain_heap h\<^sub>v \<Delta>\<^sub>v' = unchain_heap h\<^sub>v \<Delta>\<^sub>v" by auto
   from ev\<^sub>v_jump have "chained_stack \<Delta>\<^sub>v s\<^sub>v" by simp
   with ev\<^sub>v_jump have B: "unchain_stack \<Delta>\<^sub>v' s\<^sub>v = unchain_stack \<Delta>\<^sub>v s\<^sub>v" by fastforce 
@@ -225,14 +232,14 @@ lemma unchain_state_reverse [dest]: "S\<^sub>h h\<^sub>h \<V> s\<^sub>h = unchai
     \<exists>h\<^sub>v \<Delta>\<^sub>v s\<^sub>v. \<Sigma>\<^sub>v = S\<^sub>v h\<^sub>v \<Delta>\<^sub>v \<V> s\<^sub>v \<and> h\<^sub>h = unchain_heap h\<^sub>v \<Delta>\<^sub>v \<and> s\<^sub>h = unchain_stack \<Delta>\<^sub>v s\<^sub>v"
   by (induction \<Sigma>\<^sub>v) simp_all
 
-lemma unchain_lam_reverse [dest]: "Lam\<^sub>h \<Delta>\<^sub>h p\<^sub>C = unchain_closure \<Delta>\<^sub>v x \<Longrightarrow> 
-    \<exists>p\<^sub>\<Delta>. x = Lam\<^sub>v p\<^sub>\<Delta> p\<^sub>C \<and> \<Delta>\<^sub>h = unchain_env \<Delta>\<^sub>v p\<^sub>\<Delta>"
+lemma unchain_lam_reverse [dest]: "Lam\<^sub>h \<Delta>\<^sub>h p\<^sub>C n = unchain_closure \<Delta>\<^sub>v x \<Longrightarrow> 
+    \<exists>p\<^sub>\<Delta>. x = Lam\<^sub>v p\<^sub>\<Delta> p\<^sub>C n \<and> \<Delta>\<^sub>h = unchain_env \<Delta>\<^sub>v p\<^sub>\<Delta>"
   by (induction x) simp_all
 
 theorem correct\<^sub>v [simp]: "\<C> \<tturnstile> unchain_state \<Sigma>\<^sub>v \<leadsto>\<^sub>h \<Sigma>\<^sub>h \<Longrightarrow> chained_state \<Sigma>\<^sub>v \<Longrightarrow>
   \<exists>\<Sigma>\<^sub>v'. (\<C> \<tturnstile> \<Sigma>\<^sub>v \<leadsto>\<^sub>v \<Sigma>\<^sub>v') \<and> \<Sigma>\<^sub>h = unchain_state \<Sigma>\<^sub>v'"
 proof (induction "unchain_state \<Sigma>\<^sub>v" \<Sigma>\<^sub>h arbitrary: \<Sigma>\<^sub>v rule: eval\<^sub>h.induct)
-  case (ev\<^sub>h_lookup \<C> p\<^sub>\<C> x y z \<Delta>\<^sub>h v h\<^sub>h \<V> s\<^sub>h)
+  case (ev\<^sub>h_lookup \<C> p\<^sub>\<C> x y \<Delta>\<^sub>h vs v h\<^sub>h \<V> s\<^sub>h)
   then obtain h\<^sub>v \<Delta>\<^sub>v s\<^sub>v' where S: "\<Sigma>\<^sub>v = S\<^sub>v h\<^sub>v \<Delta>\<^sub>v \<V> s\<^sub>v' \<and> h\<^sub>h = unchain_heap h\<^sub>v \<Delta>\<^sub>v \<and> 
     (\<Delta>\<^sub>h, Suc p\<^sub>\<C>) # s\<^sub>h = unchain_stack \<Delta>\<^sub>v s\<^sub>v'" by fastforce
   then obtain f\<^sub>v s\<^sub>v where SF: "s\<^sub>v' = f\<^sub>v # s\<^sub>v \<and> (\<Delta>\<^sub>h, Suc p\<^sub>\<C>) = unchain_frame \<Delta>\<^sub>v f\<^sub>v \<and> 
@@ -271,8 +278,8 @@ next
     s\<^sub>h = unchain_stack \<Delta>\<^sub>v s\<^sub>v" by auto
   then obtain p\<^sub>\<Delta> where P: "f\<^sub>v = (p\<^sub>\<Delta>, Suc p\<^sub>\<C>) \<and> \<Delta>\<^sub>h = unchain_env \<Delta>\<^sub>v p\<^sub>\<Delta>" by (cases f\<^sub>v) simp_all
   with ev\<^sub>h_pushlam S have "halloc (hmap (unchain_closure \<Delta>\<^sub>v) h\<^sub>v) 
-    (unchain_closure \<Delta>\<^sub>v (Lam\<^sub>v p\<^sub>\<Delta> p\<^sub>\<C>')) = (h\<^sub>h', v)" by simp
-  then obtain h\<^sub>v' where H: "halloc h\<^sub>v (Lam\<^sub>v p\<^sub>\<Delta> p\<^sub>\<C>') = (h\<^sub>v', v) \<and> 
+    (unchain_closure \<Delta>\<^sub>v (Lam\<^sub>v p\<^sub>\<Delta> p\<^sub>\<C>' n)) = (h\<^sub>h', v)" by simp
+  then obtain h\<^sub>v' where H: "halloc h\<^sub>v (Lam\<^sub>v p\<^sub>\<Delta> p\<^sub>\<C>' n) = (h\<^sub>v', v) \<and> 
     h\<^sub>h' = hmap (unchain_closure \<Delta>\<^sub>v) h\<^sub>v'" by (metis halloc_map_inv)
   hence "h\<^sub>h' = unchain_heap h\<^sub>v' \<Delta>\<^sub>v" by simp
   with SF P have X: "S\<^sub>h h\<^sub>h' (v # \<V>) ((\<Delta>\<^sub>h, p\<^sub>\<C>) # s\<^sub>h) = 
@@ -281,30 +288,30 @@ next
     S\<^sub>v h\<^sub>v' \<Delta>\<^sub>v (v # \<V>) ((p\<^sub>\<Delta>, p\<^sub>\<C>) # s\<^sub>v)" by simp
   with S SF P X show ?case by blast
 next
-  case (ev\<^sub>h_apply \<C> p\<^sub>\<C> h\<^sub>h v\<^sub>2 \<Delta>\<^sub>h' p\<^sub>\<C>' v\<^sub>1 \<V> \<Delta>\<^sub>h s\<^sub>h)
+  case (ev\<^sub>h_apply \<C> p\<^sub>\<C> h\<^sub>h v\<^sub>2 \<Delta>\<^sub>h' p\<^sub>\<C>' n v\<^sub>1 \<V> \<Delta>\<^sub>h s\<^sub>h)
   then obtain h\<^sub>v \<Delta>\<^sub>v s\<^sub>v' where S: "\<Sigma>\<^sub>v = S\<^sub>v h\<^sub>v \<Delta>\<^sub>v (v\<^sub>1 # v\<^sub>2 # \<V>) s\<^sub>v' \<and> 
     h\<^sub>h = unchain_heap h\<^sub>v \<Delta>\<^sub>v \<and> (\<Delta>\<^sub>h, Suc p\<^sub>\<C>) # s\<^sub>h = unchain_stack \<Delta>\<^sub>v s\<^sub>v'" by fastforce
   then obtain f\<^sub>v s\<^sub>v where SF: "s\<^sub>v' = f\<^sub>v # s\<^sub>v \<and> (\<Delta>\<^sub>h, Suc p\<^sub>\<C>) = unchain_frame \<Delta>\<^sub>v f\<^sub>v \<and> 
     s\<^sub>h = unchain_stack \<Delta>\<^sub>v s\<^sub>v" by auto
   then obtain p\<^sub>\<Delta> where P: "f\<^sub>v = (p\<^sub>\<Delta>, Suc p\<^sub>\<C>) \<and> \<Delta>\<^sub>h = unchain_env \<Delta>\<^sub>v p\<^sub>\<Delta>" by (cases f\<^sub>v) simp_all
-  from ev\<^sub>h_apply S have "Lam\<^sub>h \<Delta>\<^sub>h' p\<^sub>\<C>' = unchain_closure \<Delta>\<^sub>v (hlookup h\<^sub>v v\<^sub>2)" by simp
-  then obtain p\<^sub>\<Delta>' where P': "hlookup h\<^sub>v v\<^sub>2 = Lam\<^sub>v p\<^sub>\<Delta>' p\<^sub>\<C>' \<and> \<Delta>\<^sub>h' = unchain_env \<Delta>\<^sub>v p\<^sub>\<Delta>'" by blast
-  obtain \<Delta>\<^sub>v' p\<^sub>\<Delta>'' where H: "halloc \<Delta>\<^sub>v (v\<^sub>1, p\<^sub>\<Delta>') = (\<Delta>\<^sub>v', p\<^sub>\<Delta>'')" 
-    by (cases "halloc \<Delta>\<^sub>v (v\<^sub>1, p\<^sub>\<Delta>')") simp_all
+  from ev\<^sub>h_apply S have "Lam\<^sub>h \<Delta>\<^sub>h' p\<^sub>\<C>' n = unchain_closure \<Delta>\<^sub>v (hlookup h\<^sub>v v\<^sub>2)" by simp
+  then obtain p\<^sub>\<Delta>' where P': "hlookup h\<^sub>v v\<^sub>2 = Lam\<^sub>v p\<^sub>\<Delta>' p\<^sub>\<C>' n \<and> \<Delta>\<^sub>h' = unchain_env \<Delta>\<^sub>v p\<^sub>\<Delta>'" by blast
+  obtain \<Delta>\<^sub>v' p\<^sub>\<Delta>'' where H: "halloc \<Delta>\<^sub>v ([v\<^sub>1], p\<^sub>\<Delta>') = (\<Delta>\<^sub>v', p\<^sub>\<Delta>'')" 
+    by (cases "halloc \<Delta>\<^sub>v ([v\<^sub>1], p\<^sub>\<Delta>')") simp_all
   from ev\<^sub>h_apply S SF P have C: "chain_structured h\<^sub>v \<Delta>\<^sub>v \<and> chained_closures \<Delta>\<^sub>v h\<^sub>v \<and>
     hcontains h\<^sub>v v\<^sub>1 \<and> hcontains h\<^sub>v v\<^sub>2 \<and> chained_vals h\<^sub>v \<V> \<and> chained_frame \<Delta>\<^sub>v (p\<^sub>\<Delta>, Suc p\<^sub>\<C>) \<and> 
       chained_stack \<Delta>\<^sub>v s\<^sub>v" by simp
   with H have Y: "unchain_heap h\<^sub>v \<Delta>\<^sub>v' = unchain_heap h\<^sub>v \<Delta>\<^sub>v" by fast
   from H C have "unchain_env \<Delta>\<^sub>v' p\<^sub>\<Delta> = unchain_env \<Delta>\<^sub>v p\<^sub>\<Delta>" by fastforce
   with P have W: "\<Delta>\<^sub>h = unchain_env \<Delta>\<^sub>v' p\<^sub>\<Delta>" by metis
-  from P' C have "chained_closure \<Delta>\<^sub>v (Lam\<^sub>v p\<^sub>\<Delta>' p\<^sub>\<C>')" by (metis hlookup_all)
+  from P' C have "chained_closure \<Delta>\<^sub>v (Lam\<^sub>v p\<^sub>\<Delta>' p\<^sub>\<C>' n)" by (metis hlookup_all)
   hence "chained_heap_pointer \<Delta>\<^sub>v p\<^sub>\<Delta>'" by auto
-  with H C have "unchain_env \<Delta>\<^sub>v' (Suc p\<^sub>\<Delta>'') = v\<^sub>1 # unchain_env \<Delta>\<^sub>v p\<^sub>\<Delta>'" 
+  with H C have "unchain_env \<Delta>\<^sub>v' (Suc p\<^sub>\<Delta>'') = [v\<^sub>1] # unchain_env \<Delta>\<^sub>v p\<^sub>\<Delta>'" 
     by (metis unfold_unstack_list)
-  with H P' have Z: "v\<^sub>1 # \<Delta>\<^sub>h' = unchain_env \<Delta>\<^sub>v' (Suc p\<^sub>\<Delta>'')" by simp
+  with H P' have Z: "[v\<^sub>1] # \<Delta>\<^sub>h' = unchain_env \<Delta>\<^sub>v' (Suc p\<^sub>\<Delta>'')" by simp
   from H C have "unchain_stack \<Delta>\<^sub>v' s\<^sub>v = unchain_stack \<Delta>\<^sub>v s\<^sub>v" by fast
   with SF have "s\<^sub>h = unchain_stack \<Delta>\<^sub>v' s\<^sub>v" by simp
-  with S Y Z W have X: "S\<^sub>h h\<^sub>h \<V> ((v\<^sub>1 # \<Delta>\<^sub>h', p\<^sub>\<C>') # (\<Delta>\<^sub>h, p\<^sub>\<C>) # s\<^sub>h) = 
+  with S Y Z W have X: "S\<^sub>h h\<^sub>h \<V> (([v\<^sub>1] # \<Delta>\<^sub>h', p\<^sub>\<C>') # (\<Delta>\<^sub>h, p\<^sub>\<C>) # s\<^sub>h) = 
     unchain_state (S\<^sub>v h\<^sub>v \<Delta>\<^sub>v' \<V> ((Suc p\<^sub>\<Delta>'', p\<^sub>\<C>') # (p\<^sub>\<Delta>, p\<^sub>\<C>) # s\<^sub>v))" by simp
   from ev\<^sub>h_apply P' H have "\<C> \<tturnstile> S\<^sub>v h\<^sub>v \<Delta>\<^sub>v (v\<^sub>1 # v\<^sub>2 # \<V>) ((p\<^sub>\<Delta>, Suc p\<^sub>\<C>) # s\<^sub>v) \<leadsto>\<^sub>v 
       S\<^sub>v h\<^sub>v \<Delta>\<^sub>v' \<V> ((Suc p\<^sub>\<Delta>'', p\<^sub>\<C>') # (p\<^sub>\<Delta>, p\<^sub>\<C>) # s\<^sub>v)" by simp
@@ -316,8 +323,8 @@ next
   then obtain f\<^sub>v s\<^sub>v where SF: "s\<^sub>v' = f\<^sub>v # s\<^sub>v \<and> (\<Delta>\<^sub>h, Suc p\<^sub>\<C>) = unchain_frame \<Delta>\<^sub>v f\<^sub>v \<and> 
     s\<^sub>h = unchain_stack \<Delta>\<^sub>v s\<^sub>v" by auto
   then obtain p\<^sub>\<Delta> where P: "f\<^sub>v = (p\<^sub>\<Delta>, Suc p\<^sub>\<C>) \<and> \<Delta>\<^sub>h = unchain_env \<Delta>\<^sub>v p\<^sub>\<Delta>" by (cases f\<^sub>v) simp_all
-  obtain \<Delta>\<^sub>v' p\<^sub>\<Delta>' where H: "halloc \<Delta>\<^sub>v (v, p\<^sub>\<Delta>) = (\<Delta>\<^sub>v', p\<^sub>\<Delta>')" 
-    by (cases "halloc \<Delta>\<^sub>v (v, p\<^sub>\<Delta>)") simp_all
+
+(*
   from ev\<^sub>h_pushenv S SF P H have A: "unchain_heap h\<^sub>v \<Delta>\<^sub>v' = unchain_heap h\<^sub>v \<Delta>\<^sub>v" by auto
   from ev\<^sub>h_pushenv S SF P H have B: "unchain_env \<Delta>\<^sub>v' p\<^sub>\<Delta> = unchain_env \<Delta>\<^sub>v p\<^sub>\<Delta>" by auto 
   from ev\<^sub>h_pushenv S SF P have "chained_stack \<Delta>\<^sub>v s\<^sub>v" by simp
@@ -328,6 +335,8 @@ next
   from ev\<^sub>h_pushenv H have "\<C> \<tturnstile> S\<^sub>v h\<^sub>v \<Delta>\<^sub>v (v # \<V>) ((p\<^sub>\<Delta>, Suc p\<^sub>\<C>) # s\<^sub>v) \<leadsto>\<^sub>v 
     S\<^sub>v h\<^sub>v \<Delta>\<^sub>v' \<V> ((Suc p\<^sub>\<Delta>', p\<^sub>\<C>) # s\<^sub>v)" by simp
   with S SF P X show ?case by blast
+*)
+  thus ?case by simp
 next
   case (ev\<^sub>h_return \<C> p\<^sub>\<C> h\<^sub>h \<V> \<Delta>\<^sub>h s\<^sub>h)
   then obtain h\<^sub>v \<Delta>\<^sub>v s\<^sub>v' where S: "\<Sigma>\<^sub>v = S\<^sub>v h\<^sub>v \<Delta>\<^sub>v \<V> s\<^sub>v' \<and> h\<^sub>h = unchain_heap h\<^sub>v \<Delta>\<^sub>v \<and> 
@@ -339,28 +348,28 @@ next
   from ev\<^sub>h_return have "\<C> \<tturnstile> S\<^sub>v h\<^sub>v \<Delta>\<^sub>v \<V> ((p\<^sub>\<Delta>, Suc p\<^sub>\<C>) # s\<^sub>v) \<leadsto>\<^sub>v S\<^sub>v h\<^sub>v \<Delta>\<^sub>v \<V> s\<^sub>v" by simp
   with S SF P X show ?case by blast
 next
-  case (ev\<^sub>h_jump \<C> p\<^sub>\<C> h\<^sub>h v\<^sub>2 \<Delta>\<^sub>h' p\<^sub>\<C>' v\<^sub>1 \<V> \<Delta>\<^sub>h s\<^sub>h)
+  case (ev\<^sub>h_jump \<C> p\<^sub>\<C> h\<^sub>h v\<^sub>2 \<Delta>\<^sub>h' p\<^sub>\<C>' n v\<^sub>1 \<V> \<Delta>\<^sub>h s\<^sub>h)
   then obtain h\<^sub>v \<Delta>\<^sub>v s\<^sub>v' where S: "\<Sigma>\<^sub>v = S\<^sub>v h\<^sub>v \<Delta>\<^sub>v (v\<^sub>1 # v\<^sub>2 # \<V>) s\<^sub>v' \<and> 
     h\<^sub>h = unchain_heap h\<^sub>v \<Delta>\<^sub>v \<and> (\<Delta>\<^sub>h, Suc p\<^sub>\<C>) # s\<^sub>h = unchain_stack \<Delta>\<^sub>v s\<^sub>v'" by fastforce
   then obtain f\<^sub>v s\<^sub>v where SF: "s\<^sub>v' = f\<^sub>v # s\<^sub>v \<and> (\<Delta>\<^sub>h, Suc p\<^sub>\<C>) = unchain_frame \<Delta>\<^sub>v f\<^sub>v \<and> 
     s\<^sub>h = unchain_stack \<Delta>\<^sub>v s\<^sub>v" by auto
   then obtain p\<^sub>\<Delta> where P: "f\<^sub>v = (p\<^sub>\<Delta>, Suc p\<^sub>\<C>) \<and> \<Delta>\<^sub>h = unchain_env \<Delta>\<^sub>v p\<^sub>\<Delta>" by (cases f\<^sub>v) simp_all
-  from ev\<^sub>h_jump S have "Lam\<^sub>h \<Delta>\<^sub>h' p\<^sub>\<C>' = unchain_closure \<Delta>\<^sub>v (hlookup h\<^sub>v v\<^sub>2)" by simp
-  then obtain p\<^sub>\<Delta>' where P': "hlookup h\<^sub>v v\<^sub>2 = Lam\<^sub>v p\<^sub>\<Delta>' p\<^sub>\<C>' \<and> \<Delta>\<^sub>h' = unchain_env \<Delta>\<^sub>v p\<^sub>\<Delta>'" by blast
-  obtain \<Delta>\<^sub>v' p\<^sub>\<Delta>'' where H: "halloc \<Delta>\<^sub>v (v\<^sub>1, p\<^sub>\<Delta>') = (\<Delta>\<^sub>v', p\<^sub>\<Delta>'')" 
-    by (cases "halloc \<Delta>\<^sub>v (v\<^sub>1, p\<^sub>\<Delta>')") simp_all
+  from ev\<^sub>h_jump S have "Lam\<^sub>h \<Delta>\<^sub>h' p\<^sub>\<C>' n = unchain_closure \<Delta>\<^sub>v (hlookup h\<^sub>v v\<^sub>2)" by simp
+  then obtain p\<^sub>\<Delta>' where P': "hlookup h\<^sub>v v\<^sub>2 = Lam\<^sub>v p\<^sub>\<Delta>' p\<^sub>\<C>' n \<and> \<Delta>\<^sub>h' = unchain_env \<Delta>\<^sub>v p\<^sub>\<Delta>'" by blast
+  obtain \<Delta>\<^sub>v' p\<^sub>\<Delta>'' where H: "halloc \<Delta>\<^sub>v ([v\<^sub>1], p\<^sub>\<Delta>') = (\<Delta>\<^sub>v', p\<^sub>\<Delta>'')" 
+    by (cases "halloc \<Delta>\<^sub>v ([v\<^sub>1], p\<^sub>\<Delta>')") simp_all
   from ev\<^sub>h_jump S SF P have C: "chain_structured h\<^sub>v \<Delta>\<^sub>v \<and> chained_closures \<Delta>\<^sub>v h\<^sub>v \<and>
     hcontains h\<^sub>v v\<^sub>1 \<and> hcontains h\<^sub>v v\<^sub>2 \<and> chained_vals h\<^sub>v \<V> \<and> chained_heap_pointer \<Delta>\<^sub>v p\<^sub>\<Delta> \<and> 
       chained_stack \<Delta>\<^sub>v s\<^sub>v" by simp
   with H have Y: "unchain_heap h\<^sub>v \<Delta>\<^sub>v' = unchain_heap h\<^sub>v \<Delta>\<^sub>v" by fast
-  from P' C have "chained_closure \<Delta>\<^sub>v (Lam\<^sub>v p\<^sub>\<Delta>' p\<^sub>\<C>')" by (metis hlookup_all)
+  from P' C have "chained_closure \<Delta>\<^sub>v (Lam\<^sub>v p\<^sub>\<Delta>' p\<^sub>\<C>' n)" by (metis hlookup_all)
   hence "chained_heap_pointer \<Delta>\<^sub>v p\<^sub>\<Delta>'" by simp
-  with H C have "unchain_env \<Delta>\<^sub>v' (Suc p\<^sub>\<Delta>'') = v\<^sub>1 # unchain_env \<Delta>\<^sub>v p\<^sub>\<Delta>'" 
+  with H C have "unchain_env \<Delta>\<^sub>v' (Suc p\<^sub>\<Delta>'') = [v\<^sub>1] # unchain_env \<Delta>\<^sub>v p\<^sub>\<Delta>'" 
     by (metis unfold_unstack_list)
-  with H P' have Z: "v\<^sub>1 # \<Delta>\<^sub>h' = unchain_env \<Delta>\<^sub>v' (Suc p\<^sub>\<Delta>'')" by simp
+  with H P' have Z: "[v\<^sub>1] # \<Delta>\<^sub>h' = unchain_env \<Delta>\<^sub>v' (Suc p\<^sub>\<Delta>'')" by simp
   from H C have "unchain_stack \<Delta>\<^sub>v' s\<^sub>v = unchain_stack \<Delta>\<^sub>v s\<^sub>v" by fast
   with SF have "s\<^sub>h = unchain_stack \<Delta>\<^sub>v' s\<^sub>v" by simp
-  with S Y Z have X: "S\<^sub>h h\<^sub>h \<V> ((v\<^sub>1 # \<Delta>\<^sub>h', p\<^sub>\<C>') # s\<^sub>h) = 
+  with S Y Z have X: "S\<^sub>h h\<^sub>h \<V> (([v\<^sub>1] # \<Delta>\<^sub>h', p\<^sub>\<C>') # s\<^sub>h) = 
     unchain_state (S\<^sub>v h\<^sub>v \<Delta>\<^sub>v' \<V> ((Suc p\<^sub>\<Delta>'', p\<^sub>\<C>') # s\<^sub>v))" by simp
   from ev\<^sub>h_jump P' H have "\<C> \<tturnstile> S\<^sub>v h\<^sub>v \<Delta>\<^sub>v (v\<^sub>1 # v\<^sub>2 # \<V>) ((p\<^sub>\<Delta>, Suc p\<^sub>\<C>) # s\<^sub>v) \<leadsto>\<^sub>v 
       S\<^sub>v h\<^sub>v \<Delta>\<^sub>v' \<V> ((Suc p\<^sub>\<Delta>'', p\<^sub>\<C>') # s\<^sub>v)" by simp
@@ -398,47 +407,47 @@ lemma hallock_chained_stack [simp]: "halloc \<Delta> (v, p') = (\<Delta>', p) \<
   by (induction s) simp_all
 
 lemma chained_hlookup_hcontains [elim]: "chain_structured h \<Delta> \<Longrightarrow> hcontains \<Delta> p \<Longrightarrow> 
-  hlookup \<Delta> p = (a, b) \<Longrightarrow> hcontains h a"
+  hlookup \<Delta> p = (a, b) \<Longrightarrow> list_all (hcontains h) a"
 proof -
   assume "chain_structured h \<Delta>" and "hcontains \<Delta> p" and "hlookup \<Delta> p = (a, b)"
-  hence "(\<lambda>(v, p'). p' \<le> p \<and> hcontains h v) (a, b)" by (metis hlookup_all)
+  hence "(\<lambda>(vs, p'). p' \<le> p \<and> list_all (hcontains h) vs) (a, b)" by (metis hlookup_all)
   thus ?thesis by simp
 qed
 
 lemma chain_lookup_hcontains [elim]: "chain_structured h \<Delta> \<Longrightarrow> hcontains \<Delta> p \<Longrightarrow> 
-  chain_lookup \<Delta> p x = Some v \<Longrightarrow> hcontains h v"
-proof (induction \<Delta> p x rule: chain_lookup.induct)
+  chain_lookup \<Delta> p x y = Some v \<Longrightarrow> hcontains h v"
+proof (induction \<Delta> p x y rule: chain_lookup.induct)
   case (2 \<Delta> p)
   moreover obtain a b where "hlookup \<Delta> p = (a, b)" by (cases "hlookup \<Delta> p")
   ultimately show ?case by auto
 next
-  case (3 \<Delta> p x)
+  case (3 \<Delta> p x y)
   obtain a b where A: "hlookup \<Delta> p = (a, b)" by (cases "hlookup \<Delta> p")
   from 3 have "hcontains \<Delta> p" by auto
-  with 3 A have "b \<le> p \<and> hcontains h a" using hlookup_all by fast
+  with 3 A have "b \<le> p \<and> list_all (hcontains h) a" using hlookup_all by fast
   with 3 have "hcontains \<Delta> b" by fastforce
   with 3 A show ?case by simp
 qed simp_all
 
-lemma chain_lookup_suc_hcontains [elim]: "chain_lookup \<Delta> (Suc p) x = Some v \<Longrightarrow> 
+lemma chain_lookup_suc_hcontains [elim]: "chain_lookup \<Delta> (Suc p) x y = Some v \<Longrightarrow> 
   chain_structured h \<Delta> \<Longrightarrow> hcontains \<Delta> p \<Longrightarrow> hcontains h v"
-proof (induction \<Delta> "Suc p" x arbitrary: p rule: chain_lookup.induct)
+proof (induction \<Delta> "Suc p" x y arbitrary: p rule: chain_lookup.induct)
   case (2 \<Delta> p)
   then obtain b where "hlookup \<Delta> p = (v, b)" by (cases "hlookup \<Delta> p") simp_all
-  with 2 have "b \<le> p \<and> hcontains h v" using hlookup_all by fast
+  with 2 have "b \<le> p \<and> hcontains h v" using hlookup_all by fastx
   with 2 show ?case by simp
 next
   case (3 \<Delta> p x)
   moreover then obtain a b where A: "hlookup \<Delta> p = (a, b)" by (cases "hlookup \<Delta> p")
-  moreover with 3 have "b \<le> p \<and> hcontains h a" using hlookup_all by fast
+  moreover with 3 have "b \<le> p \<and> list_all (hcontains h) a" using hlookup_all by fast
   ultimately show ?case by auto
 qed
 
 lemma chain_structured_alloc [simp]: "chained_heap_pointer \<Delta> p\<^sub>\<Delta> \<Longrightarrow> hcontains h v\<^sub>1 \<Longrightarrow> 
-  halloc \<Delta> (v\<^sub>1, p\<^sub>\<Delta>) = (\<Delta>', p\<^sub>\<Delta>') \<Longrightarrow> chain_structured h \<Delta> \<Longrightarrow> chain_structured h \<Delta>'"
+  halloc \<Delta> ([v\<^sub>1], p\<^sub>\<Delta>) = (\<Delta>', p\<^sub>\<Delta>') \<Longrightarrow> chain_structured h \<Delta> \<Longrightarrow> chain_structured h \<Delta>'"
 proof -
   assume X: "chained_heap_pointer \<Delta> p\<^sub>\<Delta>"
-  moreover assume A: "halloc \<Delta> (v\<^sub>1, p\<^sub>\<Delta>) = (\<Delta>', p\<^sub>\<Delta>')" and "chain_structured h \<Delta>" 
+  moreover assume A: "halloc \<Delta> ([v\<^sub>1], p\<^sub>\<Delta>) = (\<Delta>', p\<^sub>\<Delta>')" and "chain_structured h \<Delta>" 
     and "hcontains h v\<^sub>1"
   moreover have "p\<^sub>\<Delta> \<le> p\<^sub>\<Delta>'"
   proof (cases p\<^sub>\<Delta>)
@@ -449,26 +458,41 @@ proof -
   ultimately show ?thesis by auto
 qed
 
-lemma chain_structured_alloc_lam [simp]: "hcontains h v\<^sub>2 \<Longrightarrow> hlookup h v\<^sub>2 = Lam\<^sub>v p\<^sub>\<Delta> p\<^sub>\<C> \<Longrightarrow> 
-  chained_closures \<Delta> h \<Longrightarrow> hcontains h v\<^sub>1 \<Longrightarrow> halloc \<Delta> (v\<^sub>1, p\<^sub>\<Delta>) = (\<Delta>', p\<^sub>\<Delta>') \<Longrightarrow> 
+lemma chain_structured_alloc_lam [simp]: "hcontains h v\<^sub>2 \<Longrightarrow> hlookup h v\<^sub>2 = Lam\<^sub>v p\<^sub>\<Delta> p\<^sub>\<C> n \<Longrightarrow> 
+  chained_closures \<Delta> h \<Longrightarrow> hcontains h v\<^sub>1 \<Longrightarrow> halloc \<Delta> ([v\<^sub>1], p\<^sub>\<Delta>) = (\<Delta>', p\<^sub>\<Delta>') \<Longrightarrow> 
     chain_structured h \<Delta> \<Longrightarrow> chain_structured h \<Delta>'"
   using hlookup_all by fastforce
 
 lemma chain_structured_unfold [simp]: "chain_structured h \<Delta> \<Longrightarrow> 
-  heap_all (\<lambda>p (y, p'). p' \<le> p \<and> (y = x \<or> hcontains h y)) \<Delta>"
+  heap_all (\<lambda>p (y, p'). p' \<le> p \<and> list_all (hcontains h) y) \<Delta>"
 proof -
   have "\<And>a b. (\<lambda>p (v, p'). p' \<le> p \<and> hcontains h v) a b \<Longrightarrow> 
-    (\<lambda>p (y, p'). p' \<le> p \<and> (y = x \<or> hcontains h y)) a b" by (simp split: prod.splits)
+    (\<lambda>p (y, p'). p' \<le> p \<and> list_all (hcontains h) y) a b" by (simp split: prod.splits)
   moreover assume "chain_structured h \<Delta>"
-  ultimately show "heap_all (\<lambda>p (y, p'). p' \<le> p \<and> (y = x \<or> hcontains h y)) \<Delta>"
+  ultimately show "heap_all (\<lambda>p (y, p'). p' \<le> p \<and> list_all (hcontains h) y) \<Delta>"
     by (rule heap_all_implication)
 qed
 
 lemma eval_preserves_chained [simp]: "\<C> \<tturnstile> \<Sigma>\<^sub>v \<leadsto>\<^sub>v \<Sigma>\<^sub>v' \<Longrightarrow> chained_state \<Sigma>\<^sub>v \<Longrightarrow> chained_state \<Sigma>\<^sub>v'"
 proof (induction \<Sigma>\<^sub>v \<Sigma>\<^sub>v' rule: eval\<^sub>v.induct)
-  case (ev\<^sub>v_lookup \<C> p\<^sub>\<C> x y z \<Delta> p v h \<V> s)
-  thus ?case by (cases p) auto
-qed auto
+  case (ev\<^sub>v_lookup \<C> p\<^sub>\<C> x y \<Delta> p\<^sub>\<Delta> v h \<V> s)
+  thus ?case by (cases p\<^sub>\<Delta>) auto
+next
+  case (ev\<^sub>v_pushcon \<C> p\<^sub>\<C> n h h' v \<Delta> \<V> p\<^sub>\<Delta> s)
+  thus  ?case by autox
+next
+case (ev\<^sub>v_pushlam \<C> p\<^sub>\<C> p\<^sub>\<C>' n h p\<^sub>\<Delta> h' v \<Delta> \<V> s)
+  then show ?case by autox
+next
+  case (ev\<^sub>v_apply \<C> p\<^sub>\<C> h v\<^sub>2 p\<^sub>\<Delta>' p\<^sub>\<C>' n \<Delta> v\<^sub>1 \<Delta>' p\<^sub>\<Delta>'' \<V> p\<^sub>\<Delta> s)
+  then show ?case by autox
+next
+  case (ev\<^sub>v_pushenv \<C> p\<^sub>\<C> \<Delta> p\<^sub>\<Delta> vs p\<^sub>\<Delta>' h v \<V> s)
+  then show ?case by autox
+next
+  case (ev\<^sub>v_jump \<C> p\<^sub>\<C> h v\<^sub>2 p\<^sub>\<Delta>' p\<^sub>\<C>' n \<Delta> v\<^sub>1 \<Delta>' p\<^sub>\<Delta>'' \<V> p\<^sub>\<Delta> s)
+  then show ?case by autox
+qed simp_all
 
 lemma preserve_chained [simp]: "iter (\<tturnstile> \<C> \<leadsto>\<^sub>v) \<Sigma>\<^sub>v \<Sigma>\<^sub>v' \<Longrightarrow> chained_state \<Sigma>\<^sub>v \<Longrightarrow> chained_state \<Sigma>\<^sub>v'"
   by (induction \<Sigma>\<^sub>v \<Sigma>\<^sub>v' rule: iter.induct) simp_all
